demo/fib/Fib23proof.v
@@ -172,13 +172,13 @@ Proof.
   assert(SUCPRED := succ_pred).
 
   eapply SIRLocal.correct with (SO := eq); ss.
-  ii. clarify. unfold Fib3.prog, prog. ss. des_ifs; econs; et.
+  ii. clarify. unfold Fib3.prog, prog. ss. des_ifs; ss.
   ii. clarify. unfold owned_heap in *. des_u.
   revert m vs.
   ginit.
   { i. eapply cpn2_wcompat; eauto with paco. }
   gcofix CIH. ii.
-  step.
+  unfold Fib3.f_fib, f_fib.
   step_assume.
   unfold precond, parse_arg in *. des. des_ifs_safe. irw. rewrite T. irw.
   destruct n eqn:U.
