demo/fib/Fib45proof.v
@@ -115,7 +115,7 @@ Proof.
   assert(tau: forall E R (a: itree E R), (tau;; a) = a).
   { admit "backdoor --- relax sim_st to allow tau* before each progress". }
   eapply SIRLocal.correct with (SO := eq); ss.
-  ii. clarify. unfold Fib5.prog, prog. ss. des_ifs; econs; et.
+  ii. clarify. unfold Fib5.prog, prog. ss. des_ifs.
   { r. ii. clarify.
     assert(EQ: (Fib5.f_fib_ru oh_tgt m vs) = (f_fib_ru oh_tgt m vs)).
     { refl. }
