specIR/SIRProps.v
@@ -2,3 +2,4 @@ Require Export SIRStackproof.
 Require Export SIRHoare.
 Require Export SimSIR.
 Require Export SIRLocal.
+Require Export SIREutt.
